Arithmetic/theories/Languages/MiniGMP/Lemmas.v
@@ -31,91 +31,97 @@ Qed.
 
 
 Lemma _weakening_of_gmp_statements_semantics_1 : 
-    _weakening_of_statement_semantics_1 Empty_exp_sem _gmp_stmt_sem
+    _weakening_of_statement_semantics_1 Empty_exp_sem _gmp_stmt_sem strong_env_mem_partial_order
 .
 Proof with eauto using refl_env_mem_partial_order with rac_hint ; try easy.
     intros _ f ev₀ s ev₁ Hderiv. 
-    induction Hderiv; intros ev₀' sub Henvmem; 
+    induction Hderiv; intros ev₀' sub Hstrenvmem; apply strong_env_mem_stronger in Hstrenvmem as Henvmem; 
         epose proof (fun y => weakening_of_c_expression_semantics y ev₀) as weak_exp;
         pose proof (eq_defined_mpz_mem_partial_order ev₀ ev₀' sub Henvmem) as eq_defined ;
         pose proof (eq_mpz_env_mem_partial_order ev₀ ev₀' sub Henvmem) as  eq_mpz ;
         pose proof (mem_def_partial_order_add) as mpz_add;
         pose proof (env_partial_order_add ev₀ ev₀' sub Henvmem) as env_add.
         (* init *)
-        * exists (ev₀' <| env ; vars ::= {{x \ Def (VMpz (Some (proj1_sig sub l)))}} |> <| mstate ::= {{proj1_sig sub l \Defined 0}} |> ). split.
-            + now apply mpz_add.
-            + apply S_init with u.
-                ++ intros v Hcontra.
-                    (* the fact v is not bound to mpz location l by Ω₀ doesn't mean 
-                        that v will also not be bound to mpz location l' by Ω₀' 
-                    *) 
-                    admit.
-                ++ (* the semantic of ⊑ only ensures a defined mpz must stay the same, 
-                        but here, x points to an undefined mpz value so it can be either stay like so or
-                        be defined 
-                    *)
-                    admit.
+        * clear weak_exp eq_defined eq_mpz env_add. exists (ev₀' <| env ; vars ::= {{x \ Def (VMpz (Some (proj1_sig sub l)))}} |> <| mstate ::= {{proj1_sig sub l \Defined 0}} |> ).
+            split.
+            + admit. (* now apply mpz_add. *)
+            + clear mpz_add. apply S_init with u.
+                ++ intros v. admit.
+                ++ destruct Hstrenvmem as [e m]. now apply e in H0.
+                    
         (* clear *)
         * exists (ev₀' <| env ; vars ::= {{x\Def (VMpz None)}} |><| mstate ::= {{(proj1_sig sub) a \ Undefined u}} |>). split.
-            + now apply mpz_add.
+            + admit. (* now apply mpz_add. *)
             + apply S_clear. now apply (eq_mpz x (Some a)).
 
         (* set_i *)
-        * exists (ev₀' <| mstate ::= {{(proj1_sig sub) a \ Defined (z) ̇}} |>).  split...
+        * exists (ev₀' <| mstate ::= {{(proj1_sig sub) a \ Defined (z) ̇}} |>).  split... admit.
             apply S_set_i...
             ++ now apply (eq_mpz x (Some a)).
             ++ apply weak_exp... now exists sub.
 
         (* set_z *)
-        * exists (ev₀' <| mstate ::= {{(proj1_sig sub) a \Defined z}} |>). split...
+        * exists (ev₀' <| mstate ::= {{(proj1_sig sub) a \Defined z}} |>). split... admit.
             + apply S_set_z with (proj1_sig sub n)...
                 ++ now apply (eq_mpz x (Some a)).
                 ++ now apply (eq_mpz y (Some n)).
 
         (* get_int *)
-        *  exists (ev₀' <| env ; vars ::= fun e =>  e{x \ Def (VInt (zy ⁱⁿᵗ ir))} |>). split...
+        *  exists (ev₀' <| env ; vars ::= fun e =>  e{x \ Def (VInt (zy ⁱⁿᵗ ir))} |>). split... admit.
             apply S_get_int with (proj1_sig sub ly)... now apply (eq_mpz y (Some ly)).
         
         (* set_s *)
-        * exists (ev₀' <| mstate ::= {{(proj1_sig sub) lx \ Defined zx}} |>). split...
+        * exists (ev₀' <| mstate ::= {{(proj1_sig sub) lx \ Defined zx}} |>). split... admit.
             constructor... now apply (eq_mpz x (Some lx)).
 
         (* cmp *)
-        *  exists (ev₀' <| env ; vars ::= fun e => e{c \induced sub b} |>). 
-            split ... apply S_cmp with (proj1_sig sub lx) (proj1_sig sub ly) zx zy...
+        *  exists (ev₀' <| env ; vars ::= fun e => e{c \induced (proj1_sig sub) b} |>).  split ... admit.
+            apply S_cmp with (proj1_sig sub lx) (proj1_sig sub ly) zx zy...
                 ++ now apply (eq_mpz x (Some lx)).
                 ++ now apply (eq_mpz y (Some ly)).
                 ++ now apply cmp_induced.
         (* op *)
-        * eexists (ev₀' <| mstate ::= {{(proj1_sig sub) lr \Defined (⋄ bop zx zy)}} |>). split.
-            + now apply (mem_def_partial_order_add).
+        * eexists (ev₀' <| mstate ::= {{(proj1_sig sub) lr \Defined (⋄ bop zx zy)}} |>). split. 
+            + admit. (* now apply (mem_def_partial_order_add). *)
             + apply S_op with (proj1_sig sub lx) (proj1_sig sub ly)...
                 ++ now apply (eq_mpz x (Some lx)).
                 ++ now apply (eq_mpz y (Some ly)).
                 ++ now apply (eq_mpz r (Some lr)).
         (* scope*)
-        * admit.
+        * eexists. split.
+            + admit.
+            + apply S_Scope with ev_s ev_s. inversion H.
+                ++ rewrite <- H1. admit.
+                ++ subst. constructor. admit.
 Admitted.
 
-Definition weakening_of_gmp_statements_semantics_1 := 
-    weakening_of_statement_semantics_1 Empty_exp_sem _gmp_stmt_sem _gmp_stmt_vars _weakening_of_gmp_statements_semantics_1.
-
+(* Definition weakening_of_gmp_statements_semantics_1 := 
+    weakening_of_statement_semantics_1 Empty_exp_sem _gmp_stmt_sem _gmp_stmt_vars _weakening_of_gmp_statements_semantics_1 . *)
+ 
 Lemma _weakening_of_gmp_statements_semantics_2 : 
-    _weakening_of_statement_semantics_2 Empty_exp_sem _gmp_stmt_sem
+    _weakening_of_statement_semantics_2 Empty_exp_sem _gmp_stmt_sem env_mem_partial_order
 .
 Proof with eauto using refl_env_mem_partial_order with rac_hint ; try easy.
-    intros  exp_sem stmt_sem f ev₀ ev₀' s ev₁ [Hderiv1 Hrel].
+    intros  exp_sem stmt_sem f ev₀ ev₀' s ev₁ sub [Hderiv1 Hrel].
     generalize dependent ev₀'.
-    induction Hderiv1;  intros ev [sub Henvmem] ev' Hderiv.
+    induction Hderiv1;  intros ev Henvmem ev' Hderiv.
     - admit.     
     - admit.  
     - inversion Hderiv; subst; [|destruct bop; simpl in H1; discriminate]. split...
-        intros l v Hnotsomel. destruct (eq_dec a0 l).
-        +  subst. exfalso. admit. 
-        +  symmetry. now apply p_map_not_same.
+        intros l Hnotused. destruct (eq_dec a0 (proj1_sig sub l)).
+        + subst. exfalso. specialize (Hnotused x). apply Hnotused. clear Hnotused. destruct Henvmem as [Henv _]. specialize (Henv x).
+            inversion Henv;  try congruence. rewrite H3 in H2. inversion H2. destruct sub. 
+            apply bijective_eq_iff_f_eq in H6... now subst.
+        +  symmetry. subst. now apply p_map_not_same.
 
-    - admit.  
-    - admit.  
+    - inversion Hderiv; subst; [|destruct bop; simpl in H1; discriminate]. split...
+        intros l Hnotused.  destruct (eq_dec a0 (proj1_sig sub l)).
+        + subst. exfalso. specialize (Hnotused x). apply Hnotused. clear Hnotused. destruct Henvmem as [Henv _]. specialize (Henv x).
+            inversion Henv; subst;  try congruence.
+            ++ rewrite H3 in H4. inversion H4. destruct sub. apply bijective_eq_iff_f_eq in H8... now subst.
+            ++ now rewrite H3 in H4.
+        + symmetry. now apply p_map_not_same_eq.
+
     - admit.  
     - admit.  
     - admit.
@@ -128,33 +134,43 @@ Definition weakening_of_gmp_statements_semantics_2 :=
 
 
 Lemma _weakening_of_gmp_statements_semantics_3 : 
-    _weakening_of_statement_semantics_3 _gmp_stmt_sem _gmp_stmt_vars
+    _weakening_of_statement_semantics_3 _gmp_stmt_sem _gmp_stmt_vars exist_strong_env_mem_partial_order
 .
 Proof with eauto using refl_env_mem_partial_order with rac_hint ; try easy.
     intros Hweak ev s ev1 Hderiv. 
-    induction Hderiv; intros ev' [sub Hrel] [Henv Hmem].
-    - exists (ev' <| env ; vars ::= {{x \ Def (VMpz (Some (proj1_sig sub l)))}} |> <| mstate ::= {{proj1_sig sub l \Defined 0}} |> ).
+    induction Hderiv; intros ev' [ [sub [subrev [Hsub1 Hsub2]]] Hrel] [Henv Hmem].
+    - exists (ev' <| env ; vars ::= {{x \ Def (VMpz (Some (subrev l)))}} |> <| mstate ::= {{subrev l \Defined 0}} |> ).
         apply S_init with u.
-        + admit.
-        + destruct Hrel. specialize (H1 x). destruct H1; try congruence.
-            * destruct H3 as [[u' H3]|[ u' H3]]; congruence. 
-            * destruct H3 as [[u' H3]|[ u' H3]]; [|congruence]. admit. (* relation allows to not have the same umpz *) 
-            * admit. (* same issue with undef *)
+        + intros. specialize (H v). admit.
+        +  assert (~(dom ev - dom ev')%utils x). {
+            intros contra. apply Henv in contra. apply contra. simpl. auto.
+            }
+            apply not_in_sub_domain_prop in H1;[|apply in_domain_dec| apply in_domain_dec]. destruct H1.
+            * now epose proof (strong_reverse_dom_same ev' ev x (UMpz u) sub subrev Hsub1 Hsub2 Hrel _ H1).
+            * exfalso. apply H1. now exists (UMpz u).
     
-    - exists (ev' <| env ; vars ::= {{x\Def (VMpz None)}} |><| mstate ::= {{(proj1_sig sub) a \ Undefined u}} |>). apply S_clear.
+    -  exists (ev' <| env ; vars ::= {{x\Def (VMpz None)}} |><| mstate ::= {{subrev a \ Undefined u}} |>). apply S_clear.
         assert (~(dom ev - dom ev')%utils x). {
             intros contra. apply Henv in contra. apply contra. simpl. auto.
         }
         apply not_in_sub_domain_prop in H0;[|apply in_domain_dec| apply in_domain_dec]. destruct H0.
-        * admit. (* same issue as for c *)
+        * now epose proof (strong_reverse_dom_same ev' ev x a sub subrev Hsub1 Hsub2 Hrel _ H0).
         * exfalso. apply H0. now exists a.
 
-    - exists (ev' <| mstate ::= {{(proj1_sig sub) a \ Defined (z) ̇}} |>). apply S_set_i.
-        * admit. (* same issue as for c *)
-        * apply weakening_of_c_expression_semantics_3 with ev; [assumption|now exists sub|]. split.
-            + intros v Hdom. apply Henv in Hdom. simpl in Hdom.  
+    - exists (ev' <| mstate ::= {{subrev a \ Defined (z) ̇}} |>). apply S_set_i.
+        + assert (~(dom ev - dom ev')%utils x). {
+            intros contra. apply Henv in contra. apply contra. simpl. auto.
+        }
+        apply not_in_sub_domain_prop in H1;[|apply in_domain_dec| apply in_domain_dec]. destruct H1.
+        * now epose proof (strong_reverse_dom_same ev' ev x a sub subrev Hsub1 Hsub2 Hrel _ H1).
+        * exfalso. apply H1. now exists a.
+
+        + apply weakening_of_c_expression_semantics_3 with ev... 
+            * eexists...
+            * split. 
+                **intros v Hdom. apply Henv in Hdom. simpl in Hdom.  
                 apply Decidable.not_or in Hdom. now destruct Hdom.
-            + intros l Hdom. apply Hmem in Hdom as [l' Hdom]. simpl in Hdom.  exists l'. destruct Hdom. split... 
+                ** intros l Hdom. apply Hmem in Hdom as [l' Hdom]. simpl in Hdom.  exists l'. destruct Hdom. split... 
     - admit.  
     - admit.  
     - admit.  
@@ -167,4 +183,6 @@ Admitted.
 
 
 Definition weakening_of_gmp_statements_semantics_3 := 
-    weakening_of_statement_semantics_3 Empty_exp_sem _gmp_stmt_sem _gmp_stmt_vars weakening_of_empty_expression_semantics_3 _weakening_of_gmp_statements_semantics_3.
+    weakening_of_statement_semantics_3 Empty_exp_sem _gmp_stmt_sem _gmp_stmt_vars 
+    (weakening_of_empty_expression_semantics_3 exist_strong_env_mem_partial_order) 
+    _weakening_of_gmp_statements_semantics_3.
